Minor changes.

src/dafny/yul-verif/Examples-Yul.dfy
@@ -1,19 +1,40 @@
 
-
 include "../../../evm-dafny/src/dafny/state.dfy" 
 include "../../../evm-dafny/src/dafny/evm.dfy"
-
-include "yul-semantics.dfy"
+ 
+include "yul-semantics.dfy" 
 
 module ExamplesYul {
-
+ 
     import opened Int
     import opened Yul 
     import opened Opcode
-    import opened EvmState
+    import opened EvmState 
     import EVM
     import opened Bytecode
     import Gas
+
+    const tag_1 := 0xf 
+
+    const EX1_CODE := [
+        PUSH1, 0x0a,
+        PUSH1, 0x08,
+        PUSH1, 0x03,
+        SWAP1,
+        PUSH1, 0x0f,
+        JUMP,
+        JUMPDEST,   //  tag_2 
+        PUSH1, 0x40,
+        MSTORE,
+        STOP,
+        JUMPDEST,   //  tag_1
+        SWAP1,      
+        PUSH1, 0x01, 
+        ADD,
+        ADD,
+        SWAP1,
+        JUMP
+    ]
 
     function foo1(x: u256, y: u256): u256 
     {
@@ -32,7 +53,7 @@ module ExamplesYul {
     function foo1EVM(st:ExecutingState): State
         requires st.Capacity() >= 2
         requires st.Operands() >= 2
-        ensures st.EXECUTING?
+        ensures foo1EVM(st).EXECUTING?
     {
         var s1 := Swap(st, 1);
         var s2 := Push1(s1, 0x1);
@@ -40,9 +61,28 @@ module ExamplesYul {
         // swap + jump
     }
 
+    function {:opaque} foo1EVMJump(st:ExecutingState): (st': State)
+        requires st.Capacity() >= 2
+        requires st.Operands() >= 3
+        requires st.PC() == 0xf
+        requires st.IsJumpDest(st.Peek(2))
+        requires st.evm.code.contents == EX1_CODE
+
+        ensures st'.EXECUTING?
+        ensures st'.PC() == st.Peek(2) as nat
+        ensures st'.Operands() == st.Operands() - 2  
+    {
+        var s0 := JumpDest(st);
+        var s1 := Swap(st, 1);
+        var s2 := Push1(s1, 0x1);
+        var s3 := Add(Add(s2));
+        Jump(Swap(s3, 1))
+    }
+
      //  Let + mstore
     function foo2EVM(st:ExecutingState): State 
         requires st.Capacity() >= 4
+        requires st.PC() == 0 
         ensures foo2EVM(st).EXECUTING?
     {
         // push tag_2
@@ -60,6 +100,37 @@ module ExamplesYul {
         s6
     }
 
+     //  Let + mstore
+    function foo2EVMJump(st:ExecutingState): (st': State) 
+        requires st.Capacity() >= 6
+        requires st.PC() == 0 
+        requires st.evm.code.contents == EX1_CODE
+        // ensures foo2EVM(st).EXECUTING?
+    {
+        assert st.CodeAtPC() == PUSH1;
+        var s1 := Push1(st, 0xa);
+        var s2 := Push1(s1, 0x08);
+        var s3 := Push1(s2, 0x03);
+
+        var s4 := Push1(Swap(s3, 1), 0xf);
+        
+        assert s4.PC() == 0x9 as nat;
+        assert Jump(s4).Peek(2) == 0xa;
+        var s5 := foo1EVMJump(Jump(s4));
+
+        // check return address
+        assert s5.PC() == 0xa;
+
+        var s6 := Push1(JumpDest(s5), 0x40);
+        var s7 := MStore(s6);
+
+        assert s7.PC() == 0xe;
+
+        // assert Memory.ReadUint256(s7.evm.memory, 0x40 as nat) ==  0xc;
+        // Stop(s6)
+        s6
+    }
+
     lemma proofFoo1(x: u256, y: u256, st:ExecutingState)
         requires st.Capacity() >= 2
         requires st.Operands() >= 2
@@ -71,8 +142,37 @@ module ExamplesYul {
         //  Thanks Dafny
     }
 
+    lemma proofFoo2(st:ExecutingState)
+        requires st.Capacity() >= 4
+        // requires st.Operands() >= 2
+        // requires st.Peek(0) == x 
+        // requires st.Peek(1) == y 
+
+        // ensures foo1EVM(st).Peek(0) == foo1(x, y)
+    {
+        var x := 8;
+        var s1 := Push1(st, x as u8);
+
+        var y := 3;
+        var s2 := Swap(Push1(s1, y as u8), 1);
+
+        var z := foo1(x, y);
+        var s3 := foo1EVM(s2);
+
+        assert s3.Peek(0) == z;
+
+        //  tag_2 here 
+        var s4 := MStore(Push1(s3, 0x40));
+        assert s4.EXECUTING?;
+
+        assert Memory.ReadUint256(s4.evm.memory, 0x40 as nat) == z;
+
+        // st
+        
+    }
+
     // tag_ 1
-    function equivFoo1(x: u256, y: u256, st: ExecutingState): (r:(u256, State))
+    function {:opaque} equivFoo1(x: u256, y: u256, st: ExecutingState): (r:(u256, State))
         requires st.Capacity() >= 2
         requires st.Operands() >= 2
         ensures st.EXECUTING?
@@ -80,8 +180,9 @@ module ExamplesYul {
         requires st.Peek(1) == y 
 
         ensures r.1.EXECUTING?
-        ensures r.1.Operands() >= 1
+        ensures r.1.Operands() == st.Operands() - 1
         ensures r.1.Peek(0) == r.0
+        // ensures r.0 == add(x,add(y, 1))
     {
         (foo1(x, y), foo1EVM(st))
     }
@@ -105,7 +206,7 @@ module ExamplesYul {
 
         var (z, s3) := equivFoo1(x, y, s2);
 
-        assert s3.EXECUTING?;
+        assert Push1(s3, 0x40).EXECUTING?;
         assert s3.Operands() >= 1;
 
         //  tag_2 here 
