src/dafny/yul-verif/yul-semantics.dfy
@@ -5,14 +5,25 @@ module Yul {
 
   import opened Int
 
+  /**
+   *    Addition modulo 2^256.
+   */
   function add(x: u256, y: u256): u256
   {
     ((x as nat + y as nat) % TWO_256) as u256
   }
 
-  function mstore(x: u256, y: u256): (u256, u256) 
+  function mstore(x: u256, y: u256): (u256, u256)
   {
     (x, y)
+  }
+
+  /**
+   *    Unsigned lower than.
+   */
+  function lt(x: u256, y: u256): u256
+  {
+    if x < y then 1 else 0
   }
 
 }
